Strengthened the stuck cases so we don't need disjunctions of existentials anymore. They've been shown to be straight identity.

CertiGC/stuck.v
@@ -1,160 +1,561 @@
 Require Import RamifyCoq.CertiGC.gc_spec.
-Require Export RamifyCoq.CertiGC.gc.
-(* Require Import VST.compcert.cfrontend.Cstrategy. *)
+Require Import compcert.cfrontend.ClightBigstep.
 
-Lemma body1:
-  semax_body Vprog Gprog f_int_or_ptr_to_int int_or_ptr_to_int_spec.
+(* 
+Either comment out the two lines above or the 10 or so below. 
+They contain redundancies and will break.
+We are keeping the 10 lines below mostly just to have
+  a truly complete copy of gc_spec. It isn't surprising 
+  at all that they contain redundancies -- we imported 
+  gc_spec above!
+*)
+
+(*
+From here until the Abort on line 473 is a nearly-exact copy of gc_spec.
+Changes are on lines 127, 137, and 457.
+
+Require Export VST.veric.rmaps.
+Require Export RamifyCoq.lib.List_ext.
+Require Export RamifyCoq.graph.graph_model.
+Require Export RamifyCoq.CertiGC.GCGraph.
+Require Export RamifyCoq.CertiGC.spatial_gcgraph.
+Require Export RamifyCoq.CertiGC.env_graph_gc.
+Require Export RamifyCoq.msl_ext.iter_sepcon.
+
+Identity Coercion LGraph_LabeledGraph: LGraph >-> LabeledGraph.
+Coercion pg_lg: LabeledGraph >-> PreGraph.
+ *)
+
+Definition init_data2byte (d: init_data) : byte :=
+  match d with
+  | Init_int8 m => Byte.repr (Int.intval m)
+  | _ => Byte.one
+  end.
+
+Definition all_string_constants (sh: share) (gv: globals) : mpred :=
+  cstring sh (map init_data2byte (gvar_init v___stringlit_1)) (gv ___stringlit_1) *
+  cstring sh (map init_data2byte (gvar_init v___stringlit_2)) (gv ___stringlit_2) *
+  cstring sh (map init_data2byte (gvar_init v___stringlit_3)) (gv ___stringlit_3) *
+  cstring sh (map init_data2byte (gvar_init v___stringlit_4)) (gv ___stringlit_4) *
+  cstring sh (map init_data2byte (gvar_init v___stringlit_5)) (gv ___stringlit_5) *
+  cstring sh (map init_data2byte (gvar_init v___stringlit_6)) (gv ___stringlit_6) *
+  cstring sh (map init_data2byte (gvar_init v___stringlit_7)) (gv ___stringlit_7) *
+  cstring sh (map init_data2byte (gvar_init v___stringlit_8)) (gv ___stringlit_8) *
+  cstring sh (map init_data2byte (gvar_init v___stringlit_9)) (gv ___stringlit_9) *
+  cstring sh (map init_data2byte (gvar_init v___stringlit_10)) (gv ___stringlit_10) *
+  cstring sh (map init_data2byte (gvar_init v___stringlit_11)) (gv ___stringlit_11) *
+  cstring sh (map init_data2byte (gvar_init v___stringlit_12)) (gv ___stringlit_12) *
+  cstring sh (map init_data2byte (gvar_init v___stringlit_13)) (gv ___stringlit_13) *
+  cstring sh (map init_data2byte (gvar_init v___stringlit_14)) (gv ___stringlit_14) *
+  cstring sh (map init_data2byte (gvar_init v___stringlit_15)) (gv ___stringlit_15) *
+  cstring sh (map init_data2byte (gvar_init v___stringlit_16)) (gv ___stringlit_16).
+
+Definition test_int_or_ptr_spec :=
+ DECLARE _test_int_or_ptr
+ WITH x : val
+ PRE [ _x OF int_or_ptr_type ]
+   PROP(valid_int_or_ptr x) LOCAL(temp _x x) SEP()
+ POST [ tint ]
+   PROP()
+   LOCAL(temp ret_temp
+          (Vint (Int.repr (match x with
+                    | Vint _ => 1
+                    | _ => 0
+                    end))))
+   SEP().
+
+Definition int_or_ptr_to_int_spec :=
+  DECLARE _int_or_ptr_to_int
+  WITH x : val
+  PRE [ _x OF int_or_ptr_type ]
+    PROP(is_int I32 Signed x) LOCAL(temp _x x) SEP()
+  POST [ tint ]
+    PROP() LOCAL (temp ret_temp x) SEP().
+
+Definition int_or_ptr_to_ptr_spec :=
+  DECLARE _int_or_ptr_to_ptr
+  WITH x : val
+  PRE [ _x OF int_or_ptr_type ]
+    PROP(isptr x) LOCAL(temp _x x) SEP()
+  POST [ tptr tvoid ]
+    PROP() LOCAL (temp ret_temp x) SEP().
+
+Definition int_to_int_or_ptr_spec :=
+  DECLARE _int_to_int_or_ptr
+  WITH x : val
+  PRE [ _x OF tint ]
+    PROP(valid_int_or_ptr x)
+    LOCAL(temp _x x) SEP()
+  POST [ int_or_ptr_type ]
+    PROP() LOCAL (temp ret_temp x) SEP().
+
+Definition ptr_to_int_or_ptr_spec :=
+  DECLARE _ptr_to_int_or_ptr
+  WITH x : val
+  PRE [ _x OF tptr tvoid ]
+    PROP(valid_int_or_ptr x) LOCAL(temp _x x) SEP()
+  POST [ int_or_ptr_type ]
+    PROP() LOCAL (temp ret_temp x) SEP().
+
+Definition Is_block_spec :=
+  DECLARE _Is_block
+  WITH x : val
+  PRE [ _x OF int_or_ptr_type ]
+    PROP(valid_int_or_ptr x) LOCAL(temp _x x) SEP()
+  POST [ tint ]
+    PROP()
+    LOCAL(temp ret_temp
+               (Vint (Int.repr (match x with
+                                | Vptr _ _ => 1
+                                | _ => 0
+                                end))))
+    SEP().
+
+Definition abort_with_spec :=
+  DECLARE _abort_with
+  WITH s: val, str: list byte, sh: share
+  PRE [ _s OF tptr tschar]
+    PROP (readable_share sh) LOCAL (temp _s s) SEP (cstring sh str s)
+  POST [ tvoid ]
+    PROP (False) LOCAL() SEP().
+
+Definition IS_FROM_TYPE :=
+  ProdType (ProdType (ProdType
+                        (ProdType (ConstType share) (ConstType val))
+                        (ConstType Z)) (ConstType val)) Mpred.
+
+Definition IS_FROM_WEAK_TYPE :=
+  ProdType (ProdType (ProdType (ProdType (ProdType (ConstType share) (ConstType val)) (ConstType Z)) (ConstType val)) Mpred) (ConstType Z).
+
+(* (ProdType (ProdType (ProdType *)
+(* (ProdType (ConstType share) (ConstType val)) *)
+(* (ConstType Z)) (ConstType val)) Mpred) *)
+(* (ConstType Z). *)
+
+(* what's up with TYPE? *)
+(* see manual for spec-writing *)
+Program Definition Is_from_weak_spec :=
+  DECLARE _Is_from
+  TYPE IS_FROM_WEAK_TYPE
+  WITH sh: share, start : val, n: Z, v: val, P: mpred, m: Z
+  PRE [ _from_start OF (tptr int_or_ptr_type), (* n is pos? how did we get away without this info? add? *)
+        _from_limit OF (tptr int_or_ptr_type),
+        _v OF (tptr int_or_ptr_type)]
+    PROP ()
+    LOCAL (temp _from_start start; temp _from_limit (offset_val n start); temp _v (offset_val m start)) (* weakened here -- gave ourselves the info that it's the same block, therefore is not stuck *)
+    SEP (weak_derives P (memory_block sh n start * TT) && emp;
+         weak_derives P (valid_pointer v * TT) && emp; P)
+  POST [tint]
+    EX b: {v_in_range v start n} + {~ v_in_range v start n},
+    PROP ()
+    LOCAL (temp ret_temp (Vint (Int.repr (if b then 1 else 0))))
+    SEP (P).
+Next Obligation. Admitted.
+Next Obligation. Admitted.
+
+Definition forward_p_address
+           (p: forward_p_type) (ti: val) (f_info: fun_info) (g: LGraph) :=
+  match p with
+  | inl root_index => field_address
+                        thread_info_type
+                        [ArraySubsc (Znth root_index (live_roots_indices f_info));
+                           StructField _args] ti
+  | inr (v, n) => offset_val (WORD_SIZE * n) (vertex_address g v)
+  end.
+
+Definition limit_address g t_info from :=
+  offset_val (WORD_SIZE * gen_size t_info from) (gen_start g from).
+
+Definition next_address t_info to :=
+  field_address heap_type
+                [StructField _next;
+                   ArraySubsc (Z.of_nat to); StructField _spaces] (ti_heap_p t_info).
+
+Definition forward_spec :=
+  DECLARE _forward
+  WITH rsh: share, sh: share, gv: globals, fi: val, ti: val,
+       g: LGraph, t_info: thread_info, f_info: fun_info,
+       roots : roots_t, outlier: outlier_t,
+       from: nat, to: nat, depth: Z, forward_p: forward_p_type
+  PRE [ _from_start OF (tptr int_or_ptr_type),
+        _from_limit OF (tptr int_or_ptr_type),
+        _next OF (tptr (tptr int_or_ptr_type)),
+        _p OF (tptr int_or_ptr_type),
+        _depth OF tint]
+    PROP (readable_share rsh; writable_share sh;
+          super_compatible (g, t_info, roots) f_info outlier;
+          forward_p_compatible forward_p roots g from;
+          forward_condition g t_info from to;
+          0 <= depth <= Int.max_signed;
+          from <> to)
+    LOCAL (temp _from_start (gen_start g from);
+           temp _from_limit (limit_address g t_info from);
+           temp _next (next_address t_info to);
+           temp _p (forward_p_address forward_p ti f_info g);
+           temp _depth (Vint (Int.repr depth)))
+    SEP (all_string_constants rsh gv;
+         fun_info_rep rsh f_info fi;
+         outlier_rep outlier;
+         graph_rep g;
+         thread_info_rep sh t_info ti)
+  POST [tvoid]
+    EX g': LGraph, EX t_info': thread_info, EX roots': roots_t,
+    PROP (super_compatible (g', t_info', roots') f_info outlier;
+          roots' = upd_roots from to forward_p g roots f_info;
+          forward_relation from to (Z.to_nat depth)
+                           (forward_p2forward_t forward_p roots g) g g';
+          forward_condition g' t_info' from to;
+          thread_info_relation t_info t_info')
+    LOCAL ()
+    SEP (all_string_constants rsh gv;
+         fun_info_rep rsh f_info fi;
+         outlier_rep outlier;
+         graph_rep g';
+         thread_info_rep sh t_info' ti).
+
+Definition forward_roots_spec :=
+  DECLARE _forward_roots
+  WITH rsh: share, sh: share, gv: globals, fi: val, ti: val,
+       g: LGraph, t_info: thread_info, f_info: fun_info,
+       roots: roots_t, outlier: outlier_t, from: nat, to: nat
+  PRE [ _from_start OF (tptr int_or_ptr_type),
+        _from_limit OF (tptr int_or_ptr_type),
+        _next OF (tptr (tptr int_or_ptr_type)),
+        _fi OF (tptr tuint),
+        _ti OF (tptr thread_info_type)]
+    PROP (readable_share rsh; writable_share sh;
+          super_compatible (g, t_info, roots) f_info outlier;
+          forward_condition g t_info from to;
+          from <> to)
+    LOCAL (temp _from_start (gen_start g from);
+           temp _from_limit (limit_address g t_info from);
+           temp _next (next_address t_info to);
+           temp _fi fi; temp _ti ti)
+    SEP (all_string_constants rsh gv;
+         fun_info_rep rsh f_info fi;
+         outlier_rep outlier;
+         graph_rep g;
+         thread_info_rep sh t_info ti)
+  POST [tvoid]
+    EX g' : LGraph, EX t_info': thread_info, EX roots': roots_t,
+    PROP (super_compatible (g', t_info', roots') f_info outlier;
+          forward_roots_relation from to f_info roots g roots' g';
+          forward_condition g' t_info' from to;
+          thread_info_relation t_info t_info')
+    LOCAL ()
+    SEP (all_string_constants rsh gv;
+         fun_info_rep rsh f_info fi;
+         outlier_rep outlier;
+         graph_rep g';
+         thread_info_rep sh t_info' ti).
+
+Definition do_scan_spec :=
+  DECLARE _do_scan
+  WITH rsh: share, sh: share, gv: globals, fi: val, ti: val,
+       g: LGraph, t_info: thread_info, f_info: fun_info,
+       roots : roots_t, outlier: outlier_t,
+       from: nat, to: nat, to_index: nat
+  PRE [ _from_start OF (tptr int_or_ptr_type),
+        _from_limit OF (tptr int_or_ptr_type),
+        _scan OF (tptr int_or_ptr_type),
+        _next OF (tptr (tptr int_or_ptr_type))]
+    PROP (readable_share rsh; writable_share sh;
+          super_compatible (g, t_info, roots) f_info outlier;
+          forward_condition g t_info from to;
+          from <> to; closure_has_index g to to_index;
+          0 < gen_size t_info to; gen_unmarked g to)
+    LOCAL (temp _from_start (gen_start g from);
+           temp _from_limit (limit_address g t_info from);
+           temp _scan (offset_val (- WORD_SIZE) (vertex_address g (to, to_index)));
+           temp _next (next_address t_info to))
+    SEP (all_string_constants rsh gv;
+         fun_info_rep rsh f_info fi;
+         outlier_rep outlier;
+         graph_rep g;
+         thread_info_rep sh t_info ti)
+  POST [tvoid]
+    EX g': LGraph, EX t_info': thread_info,
+    PROP (super_compatible (g', t_info', roots) f_info outlier;
+          forward_condition g' t_info' from to;
+          do_scan_relation from to to_index g g';
+          thread_info_relation t_info t_info')
+    LOCAL ()
+    SEP (all_string_constants rsh gv;
+         fun_info_rep rsh f_info fi;
+         outlier_rep outlier;
+         graph_rep g';
+         thread_info_rep sh t_info' ti).
+
+Definition do_generation_spec :=
+  DECLARE _do_generation
+  WITH rsh: share, sh: share, gv: globals, fi: val, ti: val,
+       g: LGraph, t_info: thread_info, f_info: fun_info,
+       roots: roots_t, outlier: outlier_t, from: nat, to: nat
+  PRE [ _from OF (tptr space_type),
+        _to OF (tptr space_type),
+        _fi OF (tptr tuint),
+        _ti OF (tptr thread_info_type)]
+    PROP (readable_share rsh; writable_share sh;
+          super_compatible (g, t_info, roots) f_info outlier;
+          do_generation_condition g t_info roots f_info from to;
+          from <> to)
+    LOCAL (temp _from (space_address t_info from);
+           temp _to (space_address t_info to);
+           temp _fi fi; temp _ti ti)
+    SEP (all_string_constants rsh gv;
+         fun_info_rep rsh f_info fi;
+         outlier_rep outlier;
+         graph_rep g;
+         thread_info_rep sh t_info ti)
+  POST [tvoid]
+    EX g' : LGraph, EX t_info': thread_info, EX roots': roots_t,
+    PROP (super_compatible (g', t_info', roots') f_info outlier;
+          thread_info_relation t_info t_info';
+          do_generation_relation from to f_info roots roots' g g')
+    LOCAL ()
+    SEP (all_string_constants rsh gv;
+         fun_info_rep rsh f_info fi;
+         outlier_rep outlier;
+         graph_rep g';
+         thread_info_rep sh t_info' ti).
+
+Definition create_space_spec :=
+  DECLARE _create_space
+  WITH sh: share, s: val, n: Z, gv: globals, rsh: share
+  PRE [ _s OF (tptr space_type),
+        _n OF tuint]
+    PROP (writable_share sh;
+          readable_share rsh;
+          0 <= n < MAX_SPACE_SIZE)
+    LOCAL (temp _s s; temp _n (Vint (Int.repr n)); gvars gv)
+    SEP (all_string_constants rsh gv; data_at_ sh space_type s)
+  POST [tvoid]
+    EX p: val,
+    PROP () LOCAL ()
+    SEP (all_string_constants rsh gv;
+         malloc_token Ews (tarray int_or_ptr_type n) p;
+         data_at_ Ews (tarray int_or_ptr_type n) p;
+         data_at sh space_type (p, (p, (offset_val (WORD_SIZE * n) p))) s).
+
+Definition zero_triple: (val * (val * val)) := (nullval, (nullval, nullval)).
+
+Definition create_heap_spec :=
+  DECLARE _create_heap
+  WITH sh: share, gv: globals
+  PRE []
+    PROP (readable_share sh) LOCAL (gvars gv) SEP (all_string_constants sh gv)
+  POST [tptr heap_type]
+    EX h: val, EX p: val,
+    PROP () LOCAL (temp ret_temp h)
+    SEP (all_string_constants sh gv; malloc_token Ews heap_type h;
+         data_at Ews heap_type
+                 ((p, (p, (offset_val (WORD_SIZE * NURSERY_SIZE) p)))
+                    :: list_repeat (Z.to_nat (MAX_SPACES - 1)) zero_triple) h;
+         malloc_token Ews (tarray int_or_ptr_type NURSERY_SIZE) p;
+         data_at_ Ews (tarray int_or_ptr_type NURSERY_SIZE) p).
+
+Definition make_tinfo_spec :=
+  DECLARE _make_tinfo
+  WITH sh: share, gv: globals
+  PRE []
+    PROP (readable_share sh) LOCAL (gvars gv) SEP (all_string_constants sh gv)
+  POST [tptr thread_info_type]
+    EX t: val, EX h: val, EX p: val,
+    PROP () LOCAL (temp ret_temp t)
+    SEP (all_string_constants sh gv;
+         malloc_token Ews thread_info_type t;
+         data_at Ews thread_info_type
+                 (p, (offset_val (WORD_SIZE * NURSERY_SIZE) p,
+                      (h, list_repeat (Z.to_nat MAX_ARGS) Vundef))) t;
+         malloc_token Ews heap_type h;
+         data_at Ews heap_type
+                 ((p, (p, (offset_val (WORD_SIZE * NURSERY_SIZE) p)))
+                    :: list_repeat (Z.to_nat (MAX_SPACES - 1)) zero_triple) h;
+         malloc_token Ews (tarray int_or_ptr_type NURSERY_SIZE) p;
+         data_at_ Ews (tarray int_or_ptr_type NURSERY_SIZE) p).
+
+Definition resume_spec :=
+  DECLARE _resume
+  WITH rsh: share, sh: share, gv: globals, fi: val, ti: val,
+       g: LGraph, t_info: thread_info, f_info: fun_info,
+       roots : roots_t
+  PRE [ _fi OF (tptr tuint),
+        _ti OF (tptr thread_info_type)]
+    PROP (readable_share rsh; writable_share sh;
+          graph_thread_info_compatible g t_info;
+          graph_gen_clear g O)
+    LOCAL (temp _fi fi; temp _ti ti; gvars gv)
+    SEP (all_string_constants rsh gv;
+         fun_info_rep rsh f_info fi;
+         graph_rep g;
+         thread_info_rep sh t_info ti)
+  POST [tvoid]
+    PROP (fun_word_size f_info <= total_space (heap_head (ti_heap t_info)))
+    LOCAL ()
+    SEP (all_string_constants rsh gv;
+         fun_info_rep rsh f_info fi;
+         graph_rep g;
+         before_gc_thread_info_rep sh t_info ti).
+
+Definition garbage_collect_spec :=
+  DECLARE _garbage_collect
+  WITH rsh: share, sh: share, gv: globals, fi: val, ti: val,
+       g: LGraph, t_info: thread_info, f_info: fun_info,
+       roots : roots_t, outlier: outlier_t
+  PRE [ _fi OF (tptr tuint),
+        _ti OF (tptr thread_info_type)]
+    PROP (readable_share rsh; writable_share sh;
+          super_compatible (g, t_info, roots) f_info outlier;
+          garbage_collect_condition g t_info roots f_info;
+          safe_to_copy g)
+    LOCAL (temp _fi fi; temp _ti ti; gvars gv)
+    SEP (all_string_constants rsh gv;
+         fun_info_rep rsh f_info fi;
+         outlier_rep outlier;
+         graph_rep g;
+         before_gc_thread_info_rep sh t_info ti;
+         ti_token_rep t_info)
+  POST [tvoid]
+    EX g': LGraph, EX t_info': thread_info, EX roots': roots_t,
+    PROP (super_compatible (g', t_info', roots') f_info outlier;
+          garbage_collect_relation f_info roots roots' g g';
+          garbage_collect_condition g' t_info' roots' f_info;
+          safe_to_copy g')
+    LOCAL ()
+    SEP (all_string_constants rsh gv;
+         fun_info_rep rsh f_info fi;
+         outlier_rep outlier;
+         graph_rep g';
+         before_gc_thread_info_rep sh t_info' ti;
+         ti_token_rep t_info').
+
+Definition reset_heap_spec :=
+  DECLARE _reset_heap
+  WITH h: val
+  PRE [ _h OF (tptr heap_type)]
+    PROP () LOCAL (temp _h h) SEP ()
+  POST [tvoid]
+  PROP () LOCAL () SEP ().
+
+Definition free_heap_spec :=
+  DECLARE _free_heap
+  WITH h: val
+  PRE [ _h OF (tptr heap_type)]
+    PROP () LOCAL (temp _h h) SEP ()
+  POST [tvoid]
+  PROP () LOCAL () SEP ().
+
+Definition Gprog: funspecs :=
+  ltac:(with_library prog
+                     [test_int_or_ptr_spec;
+                      int_or_ptr_to_int_spec;
+                      int_or_ptr_to_ptr_spec;
+                      int_to_int_or_ptr_spec;
+                      ptr_to_int_or_ptr_spec;
+                      Is_block_spec;
+                      Is_from_weak_spec;
+                      abort_with_spec;
+                      forward_spec;
+                      forward_roots_spec;
+                      do_scan_spec;
+                      do_generation_spec;
+                      create_space_spec;
+                      create_heap_spec;
+                      make_tinfo_spec;
+                      resume_spec;
+                      garbage_collect_spec;
+                      reset_heap_spec;
+                      free_heap_spec]).
+
+Lemma body_is_from_weak: semax_body Vprog Gprog f_Is_from Is_from_weak_spec.
 Proof.
-  start_function.
-  unfold is_int in H.
-  destruct x eqn:?; try contradiction.
-  unfold semax.
+  (* start_function. *)
 Abort.
+  
+Lemma int_or_ptr_to_int_is_not_stuck: forall ge e le m id  i,
+    le ! id = Some (Vint i) ->
+    Clight.eval_expr ge e le m
+                     (Ecast (Etempvar id (talignas 2%N (tptr tvoid))) tint)
+                     (Vint i).
+Proof. intros; econstructor; [constructor; apply H | trivial]. Qed.
 
-Lemma body2:
-  semax_body Vprog Gprog f_int_or_ptr_to_ptr int_or_ptr_to_ptr_spec.
-Proof.
-  start_function.
-  destruct x eqn:?; try contradiction.
-Abort.
+Lemma int_or_ptr_to_ptr_is_not_stuck: forall ge e le m id b o,
+    le ! id = Some (Vptr b o) ->
+    Clight.eval_expr ge e le m
+                     (Ecast (Etempvar id (talignas 2%N (tptr tvoid)))
+                            (tptr tvoid))
+                     (Vptr b o).
+Proof. intros; econstructor; [constructor; apply H | trivial]. Qed.
 
-Lemma body3:
-  semax_body Vprog Gprog f_int_to_int_or_ptr int_to_int_or_ptr_spec.
-Proof.
-  start_function.
-  red in H.
-  destruct x; try contradiction.
-Abort.
+Lemma int_to_int_or_ptr_is_not_stuck: forall ge e le m id i,
+    le ! id = Some (Vint i) ->
+    Clight.eval_expr ge e le m
+                     (Ecast (Etempvar id tint) (talignas 2%N (tptr tvoid)))
+                     (Vint i).
+Proof. intros; econstructor; [constructor; apply H | trivial]. Qed.
 
-Lemma body4:
-  semax_body Vprog Gprog f_ptr_to_int_or_ptr ptr_to_int_or_ptr_spec.
-Proof.
-  start_function.
-  unfold semax.
-  Transparent SeparationLogicAsLogicSoundness.MainTheorem.CSHL_Def.semax.
-  (* unfold SeparationLogicAsLogicSoundness.MainTheorem.CSHL_Def.semax. *)
-Abort.
-
-Lemma body5:
-  semax_body Vprog Gprog f_Is_block Is_block_spec.
-Proof.
-  start_function.
-  unfold semax.
-Abort.
-
-Lemma int_or_ptr_to_int_is_not_stuck: forall ge e le m id id',
-    is_int I32 Signed id' ->
-    le ! id = Some id' ->
-    exists i, 
-      Clight.eval_expr ge e le m
-                       (Ecast (Etempvar id (talignas 2%N (tptr tvoid))) tint)
-                       (Vint i).
-Proof.
-  intros. destruct id'; try contradiction.
-  exists i. econstructor.
-  - constructor; apply H0.
-  - simpl; trivial.
-Qed.
-
-Lemma int_or_ptr_to_ptr_is_not_stuck: forall ge e le m id id',
-    isptr id' ->
-    le ! id = Some id' ->
-    exists b o,
-      Clight.eval_expr ge e le m
-                       (Ecast (Etempvar id (talignas 2%N (tptr tvoid))) (tptr tvoid))
-                       (Vptr b o).
-Proof.
-  intros. destruct id'; try contradiction.
-  exists b, i. econstructor.
-  - constructor; apply H0.
-  - simpl; trivial.
-Qed.
-
-Lemma int_to_int_or_ptr_is_not_stuck: forall ge e le m id id',
-    valid_int_or_ptr id' ->
-    le ! id = Some id' ->
-    (exists i, 
-        Clight.eval_expr ge e le m
-                         (Ecast (Etempvar id tint) (talignas 2%N (tptr tvoid)))
-                         (Vint i)) \/
-    (exists b o,
-        Clight.eval_expr ge e le m
-                         (Ecast (Etempvar id tint) (talignas 2%N (tptr tvoid)))
-                         (Vptr b o)).
-Proof.
-  intros; destruct id'; try contradiction.
-  - left; exists i; econstructor.
-    + constructor; apply H0.
-    + simpl; trivial.
-  - right; exists b, i; econstructor.
-    + constructor; apply H0.
-    + simpl; trivial.
-Qed.
-
-Lemma ptr_to_int_or_ptr_is_not_stuck: forall ge e le m id id' ,
-    valid_int_or_ptr id' ->
-    le ! id = Some id' ->
-    (exists i,
-        Clight.eval_expr ge e le m
-                         (Ecast (Etempvar id (tptr tvoid)) (talignas 2%N (tptr tvoid)))
-                         (Vint i)) \/
-    (exists b o,
-        Clight.eval_expr ge e le m
-                         (Ecast (Etempvar id (tptr tvoid)) (talignas 2%N (tptr tvoid)))
-                         (Vptr b o)).
-Proof.
-  intros. destruct id'; try contradiction.
-  - left; exists i; econstructor.
-    + constructor; apply H0.
-    + simpl; trivial.
-  - right; exists b, i; econstructor.
-    + constructor; apply H0.
-    + simpl; trivial.
-Qed.
+Lemma ptr_to_int_or_ptr_is_not_stuck: forall ge e le m id b o,
+    le ! id = Some (Vptr b o) ->
+    Clight.eval_expr ge e le m
+                     (Ecast (Etempvar id (tptr tvoid))
+                            (talignas 2%N (tptr tvoid)))
+                     (Vptr b o).
+Proof. intros; econstructor; [constructor; apply H | trivial]. Qed.
 
 Lemma test_int_or_ptr_is_stuck_on_ptr: forall ge e le m v id b o,
     le ! id = Some (Vptr b o) ->
     Clight.eval_expr ge e le m
-                     (Ecast
-                        (Ebinop Oand
-                                (Ecast (Etempvar id (talignas 2%N (tptr tvoid))) tint) (*why 2 and not 4?*)
-                                (Econst_int (Int.repr 1) tint) tint) tint)
+                     (Ecast (Ebinop Oand
+                     (Ecast (Etempvar id
+                     (talignas 2%N (tptr tvoid))) tint) (*why 2 and not 4?*)
+                     (Econst_int (Int.repr 1) tint) tint) tint)
                      v -> False.  
 Proof.
-  intros. inversion H0; subst. 2: inversion H1.
-  simpl in H5.
+  intros. inversion H0; subst; [|inversion H1]; simpl in H5.
   destruct v1; inversion H5; clear H5; subst.
-  + inversion H3; subst. 2: inversion H1.
-    inversion H7; subst. 2: inversion H1.
-    inversion H4; subst. 2: inversion H1.
-    rewrite H in H10. inversion H10; subst; clear H H10.
-    inversion H6; subst; clear H6.
-    destruct v2; inversion H9.
-  + clear H.
-    inversion H3; subst. 2: inversion H.
-    inversion H6; subst. 2: inversion H.
-    inversion H2; subst. 2: inversion H.
+  + inversion H3; subst; [|inversion H1];
+    inversion H7; subst; [|inversion H1];
+    inversion H4; subst; [|inversion H1];
+    rewrite H in H10; inversion H10; subst; clear H H10; inversion H6;
+      subst; clear H6; destruct v2; inversion H9.
+  + clear H;
+    inversion H3; subst; [|inversion H];
+    inversion H6; subst; [|inversion H];
+    inversion H2; subst; [|inversion H];
     destruct v1; destruct v2; inversion H8.
 Qed.
 
-(*
-Lemma is_from_is_stuck_for_ptr: forall ge e le m start limit v,
-    le ! id1 = Some (Vptr b1 o1) ->
-    le ! id2 = Some (Vptr b2 o2) ->
-    b1 <> b1 ->
-    Cstrategy.exec_stmt (Ssequence
-  (Sifthenelse (Ebinop Ole
-                 (Etempvar _from_start (tptr (talignas 2%N (tptr tvoid))))
-                 (Etempvar _v (tptr (talignas 2%N (tptr tvoid)))) tint)
-    (Sset _t'1
-      (Ecast
-        (Ebinop Olt (Etempvar _v (tptr (talignas 2%N (tptr tvoid))))
-          (Etempvar _from_limit (tptr (talignas 2%N (tptr tvoid)))) tint)
-        tbool))
-    (Sset _t'1 (Econst_int (Int.repr 0) tint)))
-  (Sreturn (Some (Etempvar _t'1 tint)))) start limit v ->
-    False
- *)      
-
-
-
+Lemma is_from_is_stuck_for_ptr: forall ge e le le2 m m2 et _from_start
+                                       _from_limit _v b1 b3 o1 o3 out,
+    le ! _from_start = Some (Vptr b1 o1) ->
+    (* le ! _from_limit = Some (Vptr b2 o2) -> *)
+    le ! _v = Some (Vptr b3 o3) ->
+    (* b1 = b2 -> *)
+    b1 <> b3 ->
+    ClightBigstep.exec_stmt ge e le m
+      (Ssequence
+        (Sifthenelse (Ebinop Ole
+          (Etempvar _from_start (tptr (talignas 2%N (tptr tvoid))))
+          (Etempvar _v (tptr (talignas 2%N (tptr tvoid)))) tint)
+            (Sset _t'1
+              (Ecast
+                (Ebinop Olt (Etempvar _v (tptr (talignas 2%N (tptr tvoid))))
+                  (Etempvar _from_limit (tptr (talignas 2%N (tptr tvoid)))) tint)
+                tbool))
+            (Sset _t'1 (Econst_int (Int.repr 0) tint)))
+        (Sreturn (Some (Etempvar _t'1 tint))))
+      et le2 m2 out -> False.
+Proof.
+  intros; inversion H2; subst;
+  (clear H2 H13; inversion H8; subst;
+   clear -H9 H H0 H1; inversion H9; subst; [|inversion H2];
+   inversion H7; subst; [|inversion H2];
+   inversion H8; subst; [|inversion H2];
+   rewrite H in H5; rewrite H0 in H6;
+   inversion H5; inversion H6; subst; clear H H0 H5 H6 H7 H8 H9;
+   simpl in H10; unfold Cop.sem_cmp in H10; simpl in H10;
+   unfold cmp_ptr in H10; simpl in H10;
+   destruct (eq_block b1 b3); [contradiction|];
+   destruct (Mem.valid_pointer m b1 (Ptrofs.unsigned o1) &&
+               Mem.valid_pointer m b3 (Ptrofs.unsigned o3))%bool; inversion H10).
+Qed.
